rocq/theories/TypeSystem/AlphaRenaming.v
@@ -5334,6 +5334,18 @@ Inductive typed_env_roots_shadow_safe
         infer_ok captured_tys ->
       typed_env_roots_shadow_safe env Ω n R Σ (EMakeClosure fname captures)
         (closure_value_ty fdef captured_tys) Σ R []
+  | TERS_CallExpr_MakeClosure : forall R R' Σ Σ' fname fdef captures
+      captured_tys args arg_roots,
+      In fdef (Program.env_fns env) ->
+      fn_name fdef = fname ->
+      fn_lifetimes fdef = 0 ->
+      check_make_closure_captures_sctx env Ω Σ captures (fn_captures fdef) =
+        infer_ok captured_tys ->
+      typed_args_roots_shadow_safe env Ω n R Σ args (fn_params fdef)
+        Σ' R' arg_roots ->
+      typed_env_roots_shadow_safe env Ω n R Σ
+        (ECallExpr (EMakeClosure fname captures) args)
+        (fn_ret fdef) Σ' R' (root_sets_union arg_roots)
   | TERS_Struct : forall R R' Σ Σ' sname lts args fields sdef roots,
       Program.lookup_struct sname env = Some sdef ->
       Datatypes.length lts = Program.struct_lifetimes sdef ->
@@ -5679,6 +5691,20 @@ Proof.
     + exact HnsR0.
     + exact HR0.
     + apply root_set_equiv_refl.
+  - intros R R' Σ Σ' fname fdef captures captured_tys args arg_roots
+      Hin Hfname Hlt Hcheck Hargs IHargs Hfresh R0 HnsR HnsR0 HR0.
+    rewrite expr_local_store_names_call_expr in Hfresh.
+    apply root_subst_images_exclude_names_app_inv in Hfresh.
+    destruct Hfresh as [_ Hfresh_args].
+    destruct (IHargs Hfresh_args R0 HnsR HnsR0 HR0)
+      as [R0' [arg_roots0 [Hargs0 [HnsR0' [HR0' Harg_roots0]]]]].
+    exists R0', (root_sets_union arg_roots0). split; [| split; [| split]].
+    + eapply TERS_CallExpr_MakeClosure; eauto.
+    + exact HnsR0'.
+    + exact HR0'.
+    + eapply root_set_equiv_trans.
+      * apply root_sets_union_equiv. exact Harg_roots0.
+      * apply root_set_equiv_sym. apply root_sets_instantiate_union_equiv.
   - intros R R' Σ Σ' sname lts args fields sdef roots Hlookup Hlen_lts
       Hlen_args Hbounds Hfields IHfields Hfresh R0 HnsR HnsR0 HR0.
     rewrite expr_local_store_names_struct in Hfresh.
@@ -7580,6 +7606,14 @@ Proof.
       Henv : root_env_sctx_keys_named ?R ?Σ |- _ =>
         exact (IH Hrn Henv)
     end.
+  - match goal with
+    | IH : root_env_no_shadow ?R ->
+        root_env_sctx_keys_named ?R ?Σ ->
+        root_env_sctx_keys_named ?R' ?Σ',
+      Hrn : root_env_no_shadow ?R,
+      Henv : root_env_sctx_keys_named ?R ?Σ |- _ =>
+        exact (IH Hrn Henv)
+    end.
   - pose proof (H H1 H2) as Hkeys1.
     assert (Hrn1 : root_env_no_shadow R1)
       by (eapply typed_env_roots_no_shadow;
@@ -7737,6 +7771,18 @@ Proof.
     + eapply root_set_sctx_roots_named_same_bindings.
       * eapply sctx_consume_path_same_bindings. eassumption.
       * eapply root_env_lookup_sctx_roots_named; eassumption.
+  - match goal with
+    | IH : root_env_no_shadow ?R ->
+        root_env_sctx_roots_named ?R ?Σ ->
+        root_env_sctx_roots_named ?R' ?Σ' /\
+        Forall (fun roots => root_set_sctx_roots_named roots ?Σ') ?arg_roots,
+      Hrn : root_env_no_shadow ?R,
+      Henv : root_env_sctx_roots_named ?R ?Σ |- _ =>
+        destruct (IH Hrn Henv) as [Henv_args Hroots_args];
+        split;
+        [ exact Henv_args
+        | apply root_sets_sctx_roots_named_union; exact Hroots_args ]
+    end.
   - match goal with
     | IH : root_env_no_shadow ?R ->
         root_env_sctx_roots_named ?R ?Σ ->
@@ -8898,6 +8944,7 @@ Lemma typed_roots_root_env_names_subset_mutual :
 Proof.
   intros env Ω n.
   apply typed_roots_ind; intros; subst; try assumption.
+  - eapply H. exact H0.
   - eapply H. exact H0.
   - eapply H. exact H0.
   - eapply root_env_names_remove_preserve_neq.
@@ -13164,6 +13211,109 @@ Proof.
     + eapply root_sets_union_rename_equiv. exact Harg_roots.
 Qed.
 
+Lemma alpha_rename_typed_env_roots_call_expr_make_closure_shadow_safe_support_forward :
+  forall env Ω n rho R Rr Σ Σr fname captures args er used used'
+    T Σ' R' roots,
+  (forall R0 R0r Σa Σb used0 e er0 used1 T0 Σa' R0' roots0,
+      In e args ->
+      typed_env_roots_shadow_safe env Ω n R0 Σa e T0 Σa' R0' roots0 ->
+      ctx_alpha rho Σa Σb ->
+      root_env_no_shadow R0 ->
+      root_env_no_shadow R0r ->
+      root_env_equiv R0r (root_env_rename rho R0) ->
+      root_env_sctx_keys_named R0 Σa ->
+      root_env_sctx_roots_named R0 Σa ->
+      rename_no_collision_on rho (root_env_names R0) ->
+      rename_no_collision_on rho (root_env_names R0') ->
+      (forall x, In x (ctx_names Σb) -> In x used0) ->
+      (forall x, In x (rename_range rho) -> In x used0) ->
+      disjoint_names (free_vars_expr e) (rename_range rho) ->
+      alpha_rename_expr rho used0 e = (er0, used1) ->
+      exists Σb' R0r' roots0r,
+        typed_env_roots_shadow_safe env Ω n R0r Σb er0 T0
+          Σb' R0r' roots0r /\
+        ctx_alpha rho Σa' Σb' /\
+        root_env_no_shadow R0r' /\
+        root_env_equiv R0r' (root_env_rename rho R0') /\
+        root_set_equiv roots0r (root_set_rename rho roots0)) ->
+  typed_env_roots_shadow_safe env Ω n R Σ
+    (ECallExpr (EMakeClosure fname captures) args) T Σ' R' roots ->
+  ctx_alpha rho Σ Σr ->
+  root_env_no_shadow R ->
+  root_env_no_shadow Rr ->
+  root_env_equiv Rr (root_env_rename rho R) ->
+  root_env_sctx_keys_named R Σ ->
+  root_env_sctx_roots_named R Σ ->
+  rename_no_collision_on rho (root_env_names R) ->
+  rename_no_collision_on rho (root_env_names R') ->
+  (forall x, In x (ctx_names Σr) -> In x used) ->
+  (forall x, In x (rename_range rho) -> In x used) ->
+  disjoint_names (free_vars_expr (ECallExpr (EMakeClosure fname captures) args))
+    (rename_range rho) ->
+  alpha_rename_expr rho used (ECallExpr (EMakeClosure fname captures) args) =
+    (er, used') ->
+  exists Σr' Rr' rootsr,
+    typed_env_roots_shadow_safe env Ω n Rr Σr er T Σr' Rr' rootsr /\
+    ctx_alpha rho Σ' Σr' /\
+    root_env_no_shadow Rr' /\
+    root_env_equiv Rr' (root_env_rename rho R') /\
+    root_set_equiv rootsr (root_set_rename rho roots).
+Proof.
+  intros env Ω n rho R Rr Σ Σr fname captures args er used used'
+    T Σ' R' roots Hexpr Htyped Hctx HnsR HnsRr HRr Hkeys Hroots
+    HnocollR HnocollR' Hctx_used Hrange_used Hdisj Hrename.
+  simpl in Hrename.
+  destruct (disjoint_names_app_l captures
+    ((fix go (args0 : list expr) : list ident :=
+        match args0 with
+        | [] => []
+        | arg :: rest => free_vars_expr arg ++ go rest
+        end) args) (rename_range rho) Hdisj) as [Hdisj_caps Hdisj_args].
+  destruct ((fix go (used0 : list ident) (args0 : list expr) {struct args0}
+              : list expr * list ident :=
+              match args0 with
+              | [] => ([], used0)
+              | arg :: rest =>
+                  let (arg', used1) := alpha_rename_expr rho used0 arg in
+                  let (rest', used2) := go used1 rest in
+                  (arg' :: rest', used2)
+              end) used args) as [argsr used_args] eqn:Hargs.
+  injection Hrename as <- <-.
+  inversion Htyped; subst.
+  destruct (alpha_rename_typed_args_roots_shadow_safe_support_forward
+    env Ω n rho R Rr Σ Σr args argsr used used_args
+    (fn_params fdef) (fn_params fdef) Σ' R' arg_roots)
+    as [Σr' [Rr' [arg_rootsr
+      [Hargs_r [Hctx_r [HnsRr' [HRr' Harg_roots]]]]]]].
+  - exact Hexpr.
+  - match goal with
+    | H : typed_args_roots_shadow_safe _ _ _ _ _ args
+          (fn_params fdef) _ _ arg_roots |- _ =>
+        exact H
+    end.
+  - exact Hctx.
+  - exact HnsR.
+  - exact HnsRr.
+  - exact HRr.
+  - exact Hkeys.
+  - exact Hroots.
+  - exact HnocollR.
+  - exact HnocollR'.
+  - exact Hctx_used.
+  - exact Hrange_used.
+  - exact Hdisj_args.
+  - apply params_alpha_refl.
+  - exact Hargs.
+  - exists Σr', Rr', (root_sets_union arg_rootsr).
+    split; [| split; [| split; [| split]]].
+    + eapply TERS_CallExpr_MakeClosure; eauto.
+      eapply check_make_closure_captures_sctx_alpha_forward; eauto.
+    + exact Hctx_r.
+    + exact HnsRr'.
+    + exact HRr'.
+    + eapply root_sets_union_rename_equiv. exact Harg_roots.
+Qed.
+
 Lemma alpha_rename_typed_env_roots_struct_shadow_safe_support_forward :
   forall env Ω n rho R Rr Σ Σr sname lts args fields er used used'
     T Σ' R' roots,
@@ -13703,7 +13853,30 @@ Proof.
         * exact Hrange_used.
         * exact Hdisj.
         * exact Hrename.
-      + inversion Htyped.
+      + destruct e; try solve [inversion Htyped].
+        eapply alpha_rename_typed_env_roots_call_expr_make_closure_shadow_safe_support_forward.
+        * intros R0 R0r Σa Σb used0 e0 er0 used1 T0 Σa' R0' roots0
+            Hin Htyped0 Halpha HnsR0 HnsR0r HR0r Hkeys0 Hroots0
+            Hnocoll0 Hnocoll0' Hcu Hru Hd Hr.
+          eapply (IH env Ω n rho R0 R0r Σa Σb e0 er0 used0 used1
+            T0 Σa' R0' roots0).
+          { pose proof (expr_size_callexpr_arg_lt (EMakeClosure i l0) l e0 Hin)
+              as Harg_lt.
+            simpl in *. lia. }
+          all: eassumption.
+        * exact Htyped.
+        * exact Hctx.
+        * exact HnsR.
+        * exact HnsRr.
+        * exact HRr.
+        * exact Hkeys.
+        * exact Hroots.
+        * exact HnocollR.
+        * exact HnocollR'.
+        * exact Hctx_used.
+        * exact Hrange_used.
+        * exact Hdisj.
+        * exact Hrename.
       + eapply (alpha_rename_typed_env_roots_struct_shadow_safe_support_forward
           env Ω n rho R Rr Σ Σr s l l0 l1 er used used' T Σ' R'
           roots).
